

Programming Languages: Functional Programming

Practicals 7. Folds, and Fold-Fusion

Shin-Cheng Mu

Autumn 2025

1. Express the following functions by *foldr*:

1. $all\ p :: List\ a \rightarrow Bool$, where $p :: a \rightarrow Bool$.
2. $elem\ z :: List\ a \rightarrow Bool$, where $z :: a$.
3. $concat :: List\ (List\ a) \rightarrow List\ a$.
4. $filter\ p :: List\ a \rightarrow List\ a$, where $p :: a \rightarrow Bool$.
5. $takeWhile\ p :: List\ a \rightarrow List\ a$, where $p :: a \rightarrow Bool$.
6. $id :: List\ a \rightarrow List\ a$.

In case you haven't seen them, $all\ p\ xs$ is `True` iff. all elements in xs satisfy p , and $elem\ z\ xs$ is `True` iff. x is a member of xs .

Solution:

1. $all\ p = foldr\ (\lambda x\ b \rightarrow p\ x \wedge b)\ True$.
2. $elem\ x = foldr\ (\lambda y\ b \rightarrow x == y \vee b)\ False$,
3. $concat = foldr\ (++)\ []$.
4. $filter\ p = foldr\ (\lambda x\ xs \rightarrow \text{if } p\ x \text{ then } x : xs \text{ else } xs)\ []$,
5. $takeWhile\ p = foldr\ (\lambda x\ xs \rightarrow \text{if } p\ x \text{ then } x : xs \text{ else } [])\ []$,
6. $id = foldr\ (:) []$.

2. Given $p :: a \rightarrow Bool$, can $dropWhile\ p :: List\ a \rightarrow List\ a$ be written as a *foldr*?

Solution: No. Consider *dropWhile even* [5, 4, 2, 1], which ought to be [5, 4, 2, 1]. Meanwhile, *dropWhile even* [4, 2, 1] = [1], and the lost elements cannot be recovered.

3. Express the following functions by *foldr*:

1. *inits* :: List *a* → List (List *a*).
2. *tails* :: List *a* → List (List *a*).
3. *perms* :: List *a* → List (List *a*).
4. *sublists* :: List *a* → List (List *a*).
5. *splits* :: List *a* → List (List *a*, List *a*).

Solution:

1. *inits* = *foldr* ($\lambda x \text{ } xss \rightarrow [] : \text{map } (x:) \text{ } xss$) [[]] .
2. *tails* = *foldr* ($\lambda x \text{ } xss \rightarrow (x : \text{head } xss) : xss$) [[]] ,
3. *perms* = *foldr* ($\lambda x \text{ } xss \rightarrow \text{concat } (\text{map } (\text{fan } x) \text{ } xss)$) [[]]
4. *sublists* = *foldr* ($\lambda x \text{ } xss \rightarrow xss \mathbin{++} \text{map } (x:) \text{ } xss$) [[]]
5. *splits* can be defined by:

$$\begin{aligned} \text{splits} &= \text{foldr } \text{spl } [([], [])] , \\ \text{where } \text{spl } x ((xs, ys) : zss) &= \\ & \quad ([], x : xs \mathbin{++} ys) : \text{map } ((x:) \times \text{id}) ((xs, ys) : zss) . \end{aligned}$$

$$\text{where } (f \times g) (x, y) = (f \text{ } x, g \text{ } y).$$

4. Prove the *foldr*-fusion theorem. To recite the theorem: given $f :: a \rightarrow b \rightarrow b$, $e :: b$, $h :: b \rightarrow c$ and $g :: a \rightarrow c \rightarrow c$, we have

$$h \cdot \text{foldr } f \text{ } e = \text{foldr } g \text{ } (h \text{ } e) ,$$

if $h (f \text{ } x \text{ } y) = g \text{ } x (h \text{ } y)$ for all x and y .

Solution: The aim is to prove that $h (\text{foldr } f \text{ } e \text{ } xs) = \text{foldr } g \text{ } (h \text{ } e) \text{ } xs$ for all xs , assuming that $h (f \text{ } x \text{ } y) = g \text{ } x (h \text{ } y)$.

Case $xs := []$:

$$\begin{aligned}
& h (\text{foldr } f \ e \ []) \\
&= h \ e \\
&= \text{foldr } g \ (h \ e) \ [] \ .
\end{aligned}$$

Case $xs := x : xs$:

$$\begin{aligned}
& h (\text{foldr } f \ e \ (x : xs)) \\
&= \{ \text{definition of foldr} \} \\
& \quad h (f \ x \ (\text{foldr } f \ e \ xs)) \\
&= \{ \text{fusion condition: } h (f \ x \ y) = g \ x \ (h \ y) \} \\
& \quad g \ x \ (h (\text{foldr } f \ e \ xs)) \\
&= \{ \text{induction} \} \\
& \quad g \ x \ (\text{foldr } g \ (h \ e) \ xs) \\
&= \{ \text{definition of foldr} \} \\
& \quad \text{foldr } g \ (h \ e) \ (x : xs) \ .
\end{aligned}$$

5. Prove the *map*-fusion rule $\text{map } f \cdot \text{map } g = \text{map } (f \cdot g)$ by *foldr*-fusion.

Solution: Since $\text{map } g$ is a *foldr*, we proceed as follows:

$$\begin{aligned}
& \text{map } f \cdot \text{map } g \\
&= \{ \text{map } g \text{ is a foldr} \} \\
& \quad \text{map } f \cdot \text{foldr } (\lambda x \ ys \rightarrow g \ x : ys) \ [] \\
&= \{ \text{foldr-fusion} \} \\
& \quad \text{foldr } (\lambda x \ ys \rightarrow f \ (g \ x) : ys) \ [] \\
&= \{ \text{definition of map as a foldr} \} \\
& \quad \text{map } (f \cdot g) \ .
\end{aligned}$$

The fusion condition is proved below:

$$\begin{aligned}
& \text{map } f \ (g \ x : ys) \\
&= \{ \text{definition map} \} \\
& \quad f \ (g \ x) : \text{map } f \ ys \ .
\end{aligned}$$

6. Prove that $\text{sum} \cdot \text{concat} = \text{sum} \cdot \text{map sum}$ by *foldr*-fusion, twice. Compare the proof with you previous proof in earlier parts of this course.

Solution:

$$\begin{aligned}
& \text{sum} \cdot \text{concat} \\
&= \text{sum} \cdot \text{foldr } (+) [] \\
&= \{ \text{foldr-fusion} \} \\
&\quad \text{foldr } (\lambda xs \ n \rightarrow \text{sum } xs + n) 0 \\
&= \{ \text{foldr-map fusion, see Exercise 7} \} \\
&\quad \text{foldr } (+) 0 \cdot \text{map sum} \\
&= \text{sum} \cdot \text{map sum} .
\end{aligned}$$

Fusion conditions for the *foldr*-fusion is

$$\text{sum } (xs ++ ys) = \text{sum } xs + \text{sum } ys ,$$

which is the key property we needed in the early part of this term to prove the same property. We have proved the property before, by induction on *xs*. We omit the proof here. (Note that we can also prove it by two more *foldr*-fusion, noting that $(++ \text{ } ys)$ is a *foldr*, and so is *sum*.)

See Exercise 7 for *foldr-map* fusion. The penultimate equality holds because $(+) \cdot \text{sum} = (\lambda xs \ n \rightarrow \text{sum } xs + n)$. Instead of *foldr-map* fusion we can also use *foldr* fusion alone. The fusion condition is $\text{sum } (\text{sum } xs : xss) = \text{sum } xs + \text{sum } xss$.

The *foldr*-fusion theorem captures the common pattern in these proofs. We only need to fill in the problem-dependent proofs.

7. The *map* fusion theorem is an instance of the *foldr-map* fusion theorem: $\text{foldr } f \ e \cdot \text{map } g = \text{foldr } (f \cdot g) \ e$.

(a) Prove the theorem.

Solution: Since *map g* is a *foldr*, we proceed as follows:

$$\begin{aligned}
& \text{foldr } f \ e \cdot \text{map } g \\
&= \{ \text{map } g \text{ is a foldr} \} \\
&\quad \text{foldr } f \ e \cdot \text{foldr } (\lambda x \ ys \rightarrow g \ x : ys) [] \\
&= \{ \text{foldr-fusion} \} \\
&\quad \text{foldr } (f \cdot g) (\text{foldr } f \ e []) \\
&= \{ \text{definition of foldr} \} \\
&\quad \text{foldr } (f \cdot g) \ e .
\end{aligned}$$

The fusion condition is proved below:

$$\begin{aligned}
& \text{foldr } f \ e \ (g \ x : ys) \\
&= \{ \text{definition foldr} \} \\
&\quad f \ (g \ x) (\text{foldr } f \ e \ ys) .
\end{aligned}$$

(b) Express $sum \cdot map (2 \times)$ as a *foldr*.

Solution:

$$\begin{aligned} & sum \cdot map (2 \times) \\ &= foldr (+) 0 \cdot map (2 \times) \\ &= \{ foldr-map \text{ fusion} \} \\ & foldr ((+) \cdot (2 \times)) 0 . \end{aligned}$$

(c) Show that $(2 \times) \cdot sum$ reduces to the same *foldr* as the one above.

Solution:

$$\begin{aligned} & (2 \times) \cdot sum \\ &= (2 \times) \cdot foldr (+) 0 \\ &= \{ foldr \text{ fusion} \} \\ & foldr ((+) \cdot (2 \times)) 0 . \end{aligned}$$

The fusion condition is

$$\begin{aligned} & 2 \times (x + y) \\ &= \{ \text{distributivity} \} \\ & 2 \times x + 2 \times y \\ &= \{ \text{definition of } (\cdot) \} \\ & ((+) \cdot (2 \times)) x (2 \times y) . \end{aligned}$$

8. Prove that $map f (xs \mathrel{++} ys) = map f xs \mathrel{++} map f ys$ by *foldr*-fusion. **Hint:** this is equivalent to $map f \cdot (\mathrel{++} ys) = (\mathrel{++} map f ys) \cdot map f$. You may need to do (any kinds of) fusion twice.

Solution: Recall that $(\mathrel{++} ys)$ is a *foldr*. Use *foldr* fusion and *foldr-map* fusion:

$$\begin{aligned} & (\mathrel{++} map f ys) \cdot map f \\ &= \{ foldr-map \text{ fusion} \} \\ & foldr ((:) \cdot f) (map f ys) \\ &= \{ foldr \text{ fusion} \} \\ & map f \cdot (\mathrel{++} ys) . \end{aligned}$$

The fusion condition of the last step is:

$$\begin{aligned} & map f (x : zs) \\ &= \{ \text{definition of } map \} \end{aligned}$$

$$\begin{aligned}
& f\ x : \text{map } f\ zs \\
= & \{ \text{definition of } (\cdot) \} \\
& ((\cdot) \cdot f)\ x\ (\text{map } f\ zs) .
\end{aligned}$$

9. Prove that $\text{length} \cdot \text{concat} = \text{sum} \cdot \text{map length}$ by fusion.

Solution: We calculate

$$\begin{aligned}
& \text{length} \cdot \text{concat} \\
= & \text{length} \cdot \text{foldr } (++)\ [] \\
= & \{ \text{foldr-fusion} \} \\
& \text{foldr } ((+) \cdot \text{length})\ 0 \\
= & \{ \mid \text{sum} = \text{foldr } (+)\ 0 \mid, \mid \text{foldr} \mid - \mid \text{map} \mid \text{fusion} \} \\
& \text{sum} \cdot \text{map length} .
\end{aligned}$$

The fusion condition is proved below:

$$\begin{aligned}
& \text{length } (xs ++ ys) \\
= & \{ (+) \text{ and } (++) \text{ homomorphic} \} \\
& \text{length } xs + \text{length } ys \\
= & \{ \text{definition of } (\cdot) \} \\
& ((+) \cdot \text{length})\ xs\ (\text{length } ys) .
\end{aligned}$$

10. Let $\text{scanr } f\ e = \text{map } (\text{foldr } f\ e) \cdot \text{tails}$. Construct, by *foldr*-fusion, an implementation of *scanr* whose number of calls to *f* is proportional to the length of the input list.

Solution: Recall that *tails* is a *foldr*:

$$\text{tails} = \text{foldr } (\lambda x\ xss \rightarrow (x : \text{head } xss) : xss)\ [[]] ,$$

We try to fuse $\text{map } (\text{foldr } f\ e)$ into *tails*. For the base value, notice that

$$\text{map } (\text{foldr } f\ e)\ [[]] = [e] .$$

To construct the step function, we work on the fusion condition:

$$\begin{aligned}
& \text{map } (\text{foldr } f\ e)\ ((x : \text{head } xss) : xss) \\
= & \{ \text{definition of } \text{map} \} \\
& \text{foldr } f\ e\ (x : \text{head } xss) : \text{map } (\text{foldr } f\ e)\ xss
\end{aligned}$$

```

= { definition of foldr }
  f x (foldr f e (head xss)) : map (foldr f e) xss
= { foldr f e (head xss) = head (map (foldr f e) xss) }
  let ys = map (foldr f e) xss
  in f x (head ys) : ys .

```

We have therefore constructed:

$$\text{scanr } f \ e = \text{foldr } (\lambda x \ y \rightarrow f \ x \ (\text{head } y)) \ [e] \ .$$

You may find the inductive definition easier to comprehend:

```

scanr f e []      = [e]
scanr f e (x : xs) = f x (head ys) : ys ,
  where ys = scanr f e xs .

```

11. Recall the function $\text{binary} :: \text{Nat} \rightarrow \text{List Nat}$ that returns the *reversed* binary representation of a natural number, for example $\text{binary } 4 = [0, 0, 1]$. Also, we talked about a function $\text{decimal} :: \text{List Nat} \rightarrow \text{Nat}$ that converts the representation back to a natural number.

(a) This time, express decimal using a foldr .

Solution:

$$\text{decimal} = \text{foldr } (\lambda d \ n \rightarrow d + 2 \times n) \ 0 \ .$$

- (b) Recall the function $\text{exp } m \ n = m^n$. Use foldr -fusion to construct step and base such that

$$\text{exp } m \cdot \text{decimal} = \text{foldr } \text{step } \text{base} \ .$$

If the fusion succeeds, we have derived a hylomorphism computing m^n :

$$\text{fastexp } m = \text{foldr } \text{step } \text{base} \cdot \text{binary} \ .$$

Solution: For the base value, we have $\text{base} = \text{exp } m \ 0 = 1$.

For the step function, we calculate

$$\begin{aligned} & \text{exp } m \ (d + 2 \times n) \\ = & \{ \text{since } m^{x+y} = m^x \times m^y \} \end{aligned}$$

$$\begin{aligned}
& \exp m d \times \exp m (2 \times n) \\
= & \{ \text{since } m^{2n} = (m^n)^2, \text{ let } \textit{square } x = x \times x \} \\
& \exp m d \times \textit{square } (\exp m n) \\
= & \{ d \text{ is either 0 or 1. Expand the definition } \} \\
& \text{if } d == 0 \text{ then } \textit{square } (\exp m n) \text{ else } m \times \textit{square } (\exp m n) .
\end{aligned}$$

Therefore we conclude

$$\exp m \cdot \textit{decimal} = \textit{foldr } (\lambda d x \rightarrow \text{if } d == 0 \text{ then } \textit{square } x \text{ else } m \times \textit{square } x) 1 .$$

12. Express $\textit{reverse} :: \text{List } a \rightarrow \text{List } a$ by a *foldr*. Let $\textit{revcat} = (++) \cdot \textit{reverse}$. Express *revcat* as a *foldr*.

Solution: $\textit{reverse} = \textit{foldr } (\lambda x xs \rightarrow xs ++ [x]) []$.

To fuse $(++)$ into *reverse*, the base value is $(++) [] = \textit{id}$. To construct the step function, we try to meet the fusion condition:

$$(++) ((\lambda x xs \rightarrow xs ++ [x]) x xs) = \textit{step } x ((++) xs) .$$

If we calculate:

$$\begin{aligned}
& (++) ((\lambda x xs \rightarrow xs ++ [x]) x xs) \\
= & (++) (xs ++ [x]) ,
\end{aligned}$$

it is hard to figure out how to proceed, since $(++)$ expects another argument. It is easier to calculate if we supply it another argument *ys*. We restart and calculate:

$$\begin{aligned}
& (++) ((\lambda x xs \rightarrow xs ++ [x]) x xs) ys \\
= & (++) (xs ++ [x]) ys \\
= & (xs ++ [x]) ++ ys \\
= & \{ (++) \text{ associative } \} \\
& xs ++ ([x] ++ ys) \\
= & \{ \text{definition of } (\cdot) \} \\
& (((++) xs) \cdot (x:)) ys \\
= & \{ \text{factor out } x, ((++) xs), \text{ and } ys \} \\
& (\lambda x f \rightarrow f \cdot (x:)) x ((++) xs) ys .
\end{aligned}$$

We conclude that

$$\textit{revcat} = \textit{foldr } (\lambda x f \rightarrow f \cdot (x:)) \textit{id} .$$

13. Fold on natural numbers.

- (a) The predicate $even :: \text{Nat} \rightarrow \text{Bool}$ yields True iff. the input is an even number. Define $even$ in terms of $foldN$.

Solution:

$$even = foldN \text{ not True} .$$

- (b) Express the identity function on natural numbers $id \ n = n$ in terms of $foldN$.

Solution:

$$id = foldN \ 1_+ \ 0 .$$

14. Fuse $even$ into $(+n)$. This way we get a function that checks whether a natural number is even after adding n .

Solution: Recall that $(+n) = foldN \ 1_+ \ n$. To fuse $even \cdot (+n)$ into one $foldN$, the base value is $even \ n$. To find out the step function, recall that $even \ (1_+ \ n) = not \ (even \ n)$. We may then conclude:

$$even \cdot (+n) = foldN \ not \ (even \ n) .$$

15. The famous Fibonacci number is defined by:

$$\begin{aligned} fib \ 0 &= 0 \\ fib \ 1 &= 1 \\ fib \ (2 + n) &= fib \ (1 + n) + fib \ n . \end{aligned}$$

The definition above, when taken directly as an algorithm, is rather slow. Define $fib2 \ n = (fib \ (1 + n), fib \ n)$. Derive an $O(n)$ implementation of $fib2$ by fusing it with $id :: \text{Nat} \rightarrow \text{Nat}$.

Solution: Recall that $id = foldN \ (1_+) \ 0$. Fusing $fib2$ into id , the base value is $fib2 \ 0 = (1, 0)$. To construct the step function we calculate

$$\begin{aligned} &fib2 \ (1_+ \ n) \\ &= (fib \ (1_+ \ (1_+ \ n)), fib \ (1_+ \ n)) \end{aligned}$$

$$\begin{aligned}
&= \{ \text{definition of } fib \} \\
&\quad (fib\ (1_+ n) + fib\ n, fib\ (1_+ n)) \\
&= (\lambda(x, y) \rightarrow (x + y, x)) (fib2\ n) .
\end{aligned}$$

Therefore we conclude that

$$fib2 = foldN\ (\lambda(x, y) \rightarrow (x + y, x))\ (1, 0) .$$

16. What are the fold fusion theorems for ETree and ITree?

Solution:

$$\begin{aligned}
h \cdot foldIT\ f\ e &= foldIT\ g\ (h\ e) \Leftarrow h\ (f\ x\ y\ z) = g\ x\ (h\ y)\ (h\ z) , \\
h \cdot foldET\ f\ k &= foldET\ g\ (h \cdot k) \Leftarrow h\ (f\ x\ y) = g\ (h\ x)\ (h\ y) .
\end{aligned}$$